SkLean/Preservation.lean
@@ -11,13 +11,17 @@ import SkLean.Ast
 import SkLean.Dsl
 import SkLean.Typing
 import Mathlib.Tactic
+import Init.Data.List.Lemmas
 
 /-
 ## Preservation of typing judgements
 
-For unevaluable expressions, the judgement is trivially held. The judgement is also trivially held for application of the \\(K\\) combinator.
+For unevaluable expressions, the judgement is trivially held.
 
-I set up some convenience lemmas to prove prservation. Type equivalence of a well-typed `K α β x y` call with the type `α` and its evaluation are established using these lemmas: if `(K α β x y) : α` and `(K α β x y).eval_once : α`, then the typing `α` is preserved.
+Preservation of typing under evaluation of `K` is proven given:
+- Evaluation of `K α β (x : α) y = x`
+- Evaluation of `(K α β x y).eval_once : α` (by `x : α` and `.eval_once = x`), then
+- Preservation of `K α β x y : α` is held
 -/
 
 lemma k_def_eq : ∀ α β x y, (Call.mk SK[(((K α) β) x)] y).eval_once = x := by
@@ -32,7 +36,11 @@ lemma s_def_eq : ∀ α β γ x y z, (Call.mk SK[(((((S α) β) γ) x) y)] z).ev
   repeat unfold NamedSkExpr.to_sk_expr
   simp
 
-lemma type_k_eval_def_eq (ctx : Ctx) : ∀ α β x y, valid_judgement ctx x α → valid_judgement ctx (Call.mk SK[(((K α) β) x)] y).eval_once α := by
+/-
+Assuming `x : α` is the easy case, but does not prove preservation alone.
+-/
+
+lemma k_x_judgement_holds_eval_once (ctx : Ctx) : ∀ α β x y, valid_judgement ctx x α → valid_judgement ctx (Call.mk SK[(((K α) β) x)] y).eval_once α := by
   intro α β x y h_t_x
   unfold Call.eval_once
   repeat unfold NamedSkExpr.to_sk_expr
@@ -41,9 +49,11 @@ lemma type_k_eval_def_eq (ctx : Ctx) : ∀ α β x y, valid_judgement ctx x α �
 
 /-
 
+Proving preservation in the general case of evaluation requires proving `K α β x y : α → (K α β x y).eval_once : α`.
+
 ## Substitution
 
-This lemma becomes tricky once substitution is required. I prove that all substitutions of `(var n) rhs` where `n ≠ 1` are noops. I also prove that all substitutions of `(var 1) rhs) = rhs`.
+This lemma becomes tricky once substitution is required. I prove that all substitutions of `(var n) rhs` where `n ≠ 1` are noops. I also prove that all substitutions of `(var 1) rhs = rhs`.
 -/
 
 lemma substitute_free_noop : ∀ rhs v n, (Var.mk n) ≠ v → Fall.substitute.substitute_e (.var v) n rhs = (.var v) := by
@@ -51,7 +61,6 @@ lemma substitute_free_noop : ∀ rhs v n, (Var.mk n) ≠ v → Fall.substitute.s
   unfold Fall.substitute.substitute_e
   simp
   intro h
-  simp_all
   match h : SkExpr.var n with
     | .var (Var.mk n') =>
       simp_all
@@ -62,7 +71,7 @@ lemma substitute_free_noop : ∀ rhs v n, (Var.mk n) ≠ v → Fall.substitute.s
     | .fall _ => contradiction
     | .call _ => contradiction
 
-lemma substitute_bound_1 : ∀ rhs, Fall.substitute.substitute_e (.var (.mk ⟨1⟩)) ⟨1⟩ rhs = rhs.with_indices_plus (.mk 1) := by
+lemma substitute_bound_1 : ∀ rhs, Fall.substitute.substitute_e (.var (.mk ⟨1⟩)) ⟨1⟩ rhs = rhs := by
   intro rhs
   unfold Fall.substitute.substitute_e
   simp
@@ -88,10 +97,10 @@ lemma substitute_s_noop : ∀ e rhs n, e = SkExpr.s (.mk) → Fall.substitute.su
   rw [h_e_not_var]
 
 /-
-I generalize this lemma to all bound variables.
+I generalize this lemmha to all bound variables.
 -/
 
-lemma n_eq_imp_bound_rhs : ∀ v n rhs, (.mk n) = v → Fall.substitute.substitute_e (.var v) n rhs = rhs.with_indices_plus n  := by
+lemma n_eq_imp_bound_rhs : ∀ v n rhs, (.mk n) = v → Fall.substitute.substitute_e (.var v) n rhs = rhs  := by
   intro v n rhs h_v_n_eq
   unfold Fall.substitute.substitute_e
   match v with
@@ -102,71 +111,144 @@ lemma n_eq_imp_bound_rhs : ∀ v n rhs, (.mk n) = v → Fall.substitute.substitu
 
 ## Combinator evaluation type preservation
 
-Now, I prove that `valid_judgement SK[K α β x y] α → valid_judgement SK[K α β x y].eval_once α`.
+Now, I prove that `valid_judgement SK[K α β x y] α → valid_judgement SK[K α β x y].eval_once α` by proving the call is well-typed with type `α`.
+
+Judgements of function application are determined to be true or false by substitution of the `∀` type of the left-hand side of the function call. This would seem to complicate the lemma once an argument to `K` like `ty_k` is provided. `ty_k` is dependent, and contains variables. However, all arguments to `K` are well-typed. This implies all variables that could show up in arguments are typed in the context. This implies all variables within the scope of an argument are bound. We can use this fact in our larger lemma.
+
+However, the judgement rule allowing `beta_eq t t' → valid_judgement e t → valid_judgement e t` further complicates matters. We defer to the later `SN` proof with `sorry` for most lemmas.
+
+A variable is bound if `ctx[(var n).n - 1] = some t`.
 -/
 
-lemma k_eval_def_eq : ∀ α β x y, (Call.mk SK[(((K α) β) x)] y).eval_once = x := by
-  intro α β x y
-  unfold Call.eval_once
-  repeat unfold NamedSkExpr.to_sk_expr
-  simp
+def is_bound (ctx : Ctx) (v : Var) :=
+  match v with
+    | .mk n => n.toNat > 0 ∧ n.toNat ≤ ctx.length
 
-lemma k_x_judgement_holds_eval_once (ctx : Ctx) : ∀ α β x y, valid_judgement ctx x α → valid_judgement ctx (Call.mk SK[(((K α) β) x)] y).eval_once α := by
-  intro α β x y t
-  rw [k_eval_def_eq α β x y]
-  exact t
+lemma all_well_typed_var_bound_iff (ctx : Ctx) : ∀ (n : BindId), (∃ t, valid_judgement ctx (.var (.mk n)) t) ↔ is_bound ctx (.mk n) := by
+  intro v
+  constructor
+  intro ⟨t_var, h_t_valid⟩
+  unfold is_bound
+  split
+  simp_all
+  cases h_t_valid
+  case beta_eq => sorry
+  case var n h_n_eq h h_valid =>
+    simp [List.getElem?_eq_some_iff] at h_valid
+    obtain ⟨h_n_length, h_has_t⟩ := h_valid
+    have h_length_pos := @List.length_pos_of_mem SkExpr t_var ctx (by rw [← h_has_t]; simp)
+    unfold GT.gt at h
+    unfold LT.lt at h
+    simp [BindId.instLT] at h
+    simp [h]
+    calc
+      n.toNat = (n.toNat - 1) + 1 := (by simp [@Nat.sub_one_add_one n.toNat (by linarith)])
+      _ ≤ ctx.length        := (by linarith)
+  intro h_is_bound
+  simp [is_bound] at h_is_bound
+  use ctx[v.toNat - 1]
+  obtain ⟨h_n_pos, h₂⟩ := h_is_bound
+  exact valid_judgement.var ctx v ctx[v.toNat - 1] (by simp [GT.gt]; unfold LT.lt; simp [BindId.instLT]; exact h_n_pos) (by simp)
 
-lemma k_judgement_x_imp_judgement_call {m n : ℕ} (ctx : Ctx) : ∀ α β x y, valid_judgement ctx α SK[Type m] → valid_judgement ctx β SK[Type n] → valid_judgement (β :: α :: ctx) x α → valid_judgement ctx SK[((((K α) β) x) y)] α := by
+lemma shift_indices_bound_noop (ctx : Ctx) : ∀ v_n shift_by, is_bound ctx (.mk v_n) → (SkExpr.var (.mk v_n)).with_indices_plus shift_by (ctx.length) = (SkExpr.var (.mk v_n)) := by
+  intro v_n shift_by h_is_bound
+  simp [SkExpr.with_indices_plus]
+  intro h_is_bound'
+  sorry
+
+lemma all_e_well_typed_bound (ctx : Ctx) : ∀ (e : SkExpr) t shift_by depth, depth = ctx.length → valid_judgement ctx e t → e.with_indices_plus shift_by depth = e := by
+  intro e t shift_by depth h_depth_valid h_judgement_t
+  match h : e with
+    | .k _ =>
+      simp [SkExpr.with_indices_plus]
+    | .s _ =>
+    simp [SkExpr.with_indices_plus]
+    | .prp _ =>
+      simp [SkExpr.with_indices_plus]
+    | .ty _ =>
+      simp [SkExpr.with_indices_plus]
+    | .fall (.mk bind_ty body) =>
+      unfold SkExpr.with_indices_plus
+      simp
+      cases h_judgement_t
+      case fall t_bind_ty t_body h_t_bind_ty h_t_body h_t_rfl =>
+        simp [Fall.bind_ty] at h_t_bind_ty
+        simp [Fall.body] at h_t_body
+        have h_depth : depth + 1 = (bind_ty :: ctx).length := by
+          simp [h_depth_valid]
+        constructor
+        simp [all_e_well_typed_bound (bind_ty :: ctx) bind_ty t_bind_ty shift_by (depth + 1) h_depth h_t_bind_ty]
+        simp [all_e_well_typed_bound (bind_ty :: ctx) body t_body shift_by (depth + 1) h_depth h_t_body]
+      case beta_eq => sorry
+    | .call (.mk lhs rhs) =>
+      unfold SkExpr.with_indices_plus
+      simp
+      cases h_judgement_t
+      case call t_lhs h_t_lhs h_t_rhs h_t_eq =>
+        simp [all_e_well_typed_bound ctx lhs (.fall t_lhs) shift_by (depth) h_depth_valid h_t_lhs]
+        simp [all_e_well_typed_bound ctx rhs t_lhs.bind_ty shift_by (depth) h_depth_valid h_t_rhs]
+      case beta_eq => sorry
+    | .var (.mk n) =>
+      have h₀ := h_judgement_t
+      cases h_judgement_t
+      case beta_eq => sorry
+      case var h_idx_valid =>
+        have h_bound := (all_well_typed_var_bound_iff ctx n).mp (by
+          use t
+        )
+        unfold is_bound at h_bound
+        simp at h_bound
+        rw [h_depth_valid]
+        exact shift_indices_bound_noop n shift_by (ctx.length) (by sorry)
+
+/-
+Using the fact that all variables that are well-typed are bound, we can say that with_indices_plus preserves the values of the variable. This concludes our lemma of preservation of `K α β x y : α`.
+-/
+
+lemma k_judgement_x_imp_judgement_call {m n : ℕ} (ctx : Ctx) : ∀ α β x y, valid_judgement ctx α SK[Type m] → valid_judgement ctx β SK[Type n] → valid_judgement ctx x α → valid_judgement ctx SK[((((K α) β) x) y)] α := by
   intro α β x y t_α t_β t_x
-  unfold NamedSkExpr.to_sk_expr at t_α
-  unfold NamedSkExpr.to_sk_expr at t_β
+  simp [NamedSkExpr.to_sk_expr] at t_α
+  simp [NamedSkExpr.to_sk_expr] at t_β
   apply valid_judgement.call ctx (Call.mk SK[(((K α) β) x)] y) α (.mk β α)
-  unfold Call.lhs
-  simp
+  simp [Call.lhs]
   apply valid_judgement.call ctx (Call.mk SK[((K α) β)] x) SK[∀ y : β, α] (.mk α SK[∀ y : β, α])
-  unfold Call.lhs
-  simp
-  apply valid_judgement.call ctx (Call.mk SK[(K α)] β) SK[∀ x : α, ∀ y : β, α] (.mk SK[Type n] SK[∀ x : α, ∀ y : β, α])
-  unfold Call.lhs
-  simp
-  apply valid_judgement.call ctx (Call.mk SK[K] α) SK[∀ β : (Type n), ∀ x : α, ∀ y : β, α] ty_k_fall
-  unfold Call.lhs
-  simp
+  simp [Call.lhs]
+  apply valid_judgement.call ctx (Call.mk SK[(K α)] β) SK[∀ x : α, ∀ y : β, α] (.mk SK[Type n] (.fall (Fall.mk α (.fall (.mk (.var (.mk ⟨3⟩)) α)))))
+  simp [Call.lhs]
+  apply valid_judgement.call ctx (Call.mk SK[K] α) SK[∀ β : (Type n), ∀ x : α, ∀ y : #β, α] ty_k_fall
+  simp [Call.lhs]
   rw [← ty_k_def_eq]
   exact valid_judgement.k ctx .mk (ty_k) m n rfl
-  unfold Fall.bind_ty
-  unfold ty_k_fall
-  simp
-  unfold Call.rhs
-  simp
+  simp [Fall.bind_ty]
+  simp [ty_k_fall]
+  simp [Call.rhs]
   exact t_α
-  repeat unfold NamedSkExpr.to_sk_expr
-  unfold Fall.substitute
-  unfold ty_k_fall
-  simp
-  simp [substitute_ty_noop]
-  unfold Fall.substitute.substitute_e
-  simp [substitute_ty_noop]
-  unfold Fall.substitute.substitute_e
-  unfold BindId.succ
-  simp
-  simp [n_eq_imp_bound_rhs]
-  unfold Fall.substitute.substitute_e
-  unfold BindId.succ
-  simp
-  simp [n_eq_imp_bound_rhs]
-  simp [substitute_free_noop]
-  unfold Call.rhs
-  simp
-  unfold SkExpr.with_indices_plus
-  simp
-  unfold Fall.body
-  simp
+  simp [NamedSkExpr.to_sk_expr]
+  simp [Call.rhs]
+  simp [ty_k_fall]
+  simp [Fall.body]
+  simp [Fall.substitute]
+  simp [Fall.substitute.substitute_e]
+  simp [BindId.succ]
+  simp [shift_indices_bound_noop]
+  sorry
+  simp [Call.rhs]
+  simp [NamedSkExpr.to_sk_expr]
+  simp [Fall.bind_ty]
+  exact t_β
+  simp [NamedSkExpr.to_sk_expr]
+  simp [Call.rhs]
+  simp [Fall.substitute]
+  simp [Fall.substitute.substitute_e]
+  simp [BindId.succ]
+  simp [Fall.body]
   
+  sorry
+  sorry
   sorry
 
 /-
-I do the same for S
+I do the same for \\(S\\).
 -/
 
 lemma judgement_holds_eval_once (ctx : Ctx) : ∀ (call : Call) (t : SkExpr), valid_judgement ctx (.call call) t ↔ valid_judgement ctx call.eval_once t := by
